HOL/DataStrs/Quicksort_Func2.thy
@@ -51,48 +51,26 @@ lemma quicksort_sorts:
   @let "xs3 = quicksort xs l r"
   @case "l \<ge> r"
   @have "l < r \<and> r < length xs"
-  @have "p - 1 < length xs"
-  @case "l < p - 1" @with
-    @case "p = 0"
-    @case "p + 1 < r" @with
-      @have "p + 1 < length xs"
-      @have "sorted (sublist' l p xs3)" @with
-        @have "p - 1 - l < r - l" @with @have "p - 1 < r" @end
-        @apply_induct_hyp "p - 1 - l" l "p - 1" xs1
-      @end
-      @have "sorted (sublist' (p + 1) (r + 1) xs3)" @with
-        @have "r - (p + 1) < r - l"
-        @apply_induct_hyp "r - (p + 1)" "p + 1" r xs2
-      @end
-      @have "sorted (sublist' l p xs3)"
-      @have "\<forall>x\<in>set (sublist' l p xs3). x \<le> xs3 ! p"
-      @have "\<forall>x\<in>set (sublist' (p + 1) (r + 1) xs3). x \<ge> xs3 ! p"
-    @end
-    @have "sorted (sublist' l p xs3)" @with
+  @have "sorted (sublist' l p xs3)" @with
+    @case "p = 0" @then
+    @case "l < p - 1" @with
       @have "p - 1 - l < r - l" @with @have "p - 1 < r" @end
       @apply_induct_hyp "p - 1 - l" l "p - 1" xs1
     @end
-    @have "sorted (sublist' (p + 1) (r + 1) xs3)"
-    @have "\<forall>x\<in>set (sublist' l p xs3). x \<le> xs3 ! p"
-    @have "\<forall>x\<in>set (sublist' (p + 1) (r + 1) xs3). x \<ge> xs3 ! p"
+    @have "p = p - 1 + 1"
   @end
-  @case "p + 1 < r" @with
-    @have "p + 1 < length xs"
-    @have "sorted (sublist' (p + 1) (r + 1) xs3)" @with
+  @have "sorted (sublist' (p + 1) (r + 1) xs3)" @with
+    @case "p + 1 < r" @with
       @have "r - (p + 1) < r - l"
       @apply_induct_hyp "r - (p + 1)" "p + 1" r xs2
     @end
-    @have "sorted (sublist' l p xs3)" @with
-      @case "p = 0" @have "p = p - 1 + 1" @end
-    @have "sorted (sublist' (p + 1) (r + 1) xs3)"
-    @have "\<forall>x\<in>set (sublist' l p xs3). x \<le> xs3 ! p"
-    @have "\<forall>x\<in>set (sublist' (p + 1) (r + 1) xs3). x \<ge> xs3 ! p"
   @end
-  @have "sorted (sublist' l p xs3)" @with
-    @case "p = 0" @have "p = p - 1 + 1" @end
-  @have "sorted (sublist' (p + 1) (r + 1) xs3)"
-  @have "\<forall>x\<in>set (sublist' l p xs3). x \<le> xs3 ! p"
-  @have "\<forall>x\<in>set (sublist' (p + 1) (r + 1) xs3). x \<ge> xs3 ! p"  
+  @have "\<forall>x\<in>set (sublist' l p xs3). x \<le> xs3 ! p" @with
+    @case "l < p - 1" @with @case "p = 0" @end
+  @end
+  @have "\<forall>x\<in>set (sublist' (p + 1) (r + 1) xs3). x \<ge> xs3 ! p" @with
+    @case "p = 0" @case "p + 1 < r"
+  @end
 @qed
 setup {* add_forward_prfstep_cond @{thm quicksort_sorts} [with_term "quicksort ?xs ?l ?r"] *}
 
